src/syntax/FStar.Syntax.Syntax.fs
@@ -709,7 +709,6 @@ let t_bv        = tconst PC.bv_lid
 let t_fv        = tconst PC.fv_lid
 let t_norm_step = tconst PC.norm_step_lid
 let t_tactic_unit = mk_Tm_app (mk_Tm_uinst (tabbrev PC.tactic_lid) [U_zero]) [as_arg t_unit] None Range.dummyRange
-let t_tac_unit    = mk_Tm_app (mk_Tm_uinst (tabbrev PC.u_tac_lid) [U_zero]) [as_arg t_unit] None Range.dummyRange
 let t_list_of t = mk_Tm_app (mk_Tm_uinst (tabbrev PC.list_lid) [U_zero]) [as_arg t] None Range.dummyRange
 let t_option_of t = mk_Tm_app (mk_Tm_uinst (tabbrev PC.option_lid) [U_zero]) [as_arg t] None Range.dummyRange
 let t_tuple2_of t1 t2 = mk_Tm_app (mk_Tm_uinst (tabbrev PC.lid_tuple2) [U_zero;U_zero]) [as_arg t1; as_arg t2] None Range.dummyRange
